#+title:  Chapter 7
#+author: Reinhard Stahn
#+setupfile: ./inc/setupfile.org
#+include: ./inc/latex-macros.org
#+property: header-args:sage :session *sage-chapter-7* :tangle chapter_7.sage
#+property: header-args:python :session *py-chapter-7* :tangle chapter_7.py

#+toc: headlines 2

* Setup
** Imports
#+begin_src sage
  from utils import commutator as com
  from utils_sage import Z, H, Ry, Rz
#+end_src

** Harmonic Oscillator
To simplify calculations we will use unit-less expressions. To do this let $\tilde{x}$,
$\tilde{p}$, etc denote physical quantities /with/ units and denote the unit-less versions
without the tilde, such that e.g.

<<unitless-position-and-momentum>>
$$
  \tilde{x} = \sqrt{\frac{\hbar}{m\omega}} \; x, \quad \tilde{p} = \sqrt{m\omega\hbar} \; p .
$$

Note that this implies $p=-\ii\partial_x$. The effect on $H$ and $a$ is the same as
setting $m=\hbar=\omega=1$ (we have e.g. $H=p^2/2+x^2/2$).

In this chapter let us use the python based computer algebra system [[https://www.sagemath.org/][sage]] to solve the
exercises (some of them). For this reason we define momentum and position operator in code
as follows:

#+name: position-momentum-operator
#+begin_src sage
  R.<x> = QQbar[]
  W = DifferentialWeylAlgebra(R)
  (x, dx) = W.gens()
  p = -i*dx
#+end_src

Having this we can define the Hamiltonian $H$ of the one-dimensional harmonic oscillator
and the corresponding annihilation ($a$), and creation operator ($a^\dagger$):

#+name: commutator-ladder-operators
#+begin_src sage
  H_qho = p^2 / 2 + x^2 / 2

  a = (x + i*p) / sqrt(2)
  ad = (x - i*p) / sqrt(2)
#+end_src

Some basic sanity checks:

#+name: commutator-ladder-operators-checks
#+begin_src sage :results replace :tangle no :cache yes
  assert com(x, p) == i
  assert com(a, ad) == 1
  "PASSED"
#+end_src

#+RESULTS[7274798eb8e917891bbfa50d7dfa80ec1b7a9b47]: commutator-ladder-operators-checks
: 'PASSED'

Note that from [[unitless-position-and-momentum][above]] we get

<<unitless-hamiltonian-and-annihilator>>
$$
  \tilde{H} = \hbar\omega H, \quad \tilde{a} = a .
$$

For convenience let us also define the number operator $N=a^\dagger a = H-1/2$. Clearly
the number operator has the same eigenstates as $H$. The corresponding eigenvalues are
shifted by $1/2$.

<<spectrum-harmonic-oscillator-1d>>
- Theorem (Spectrum of 1D Harmonic Oscillator) :: Let

  $$ \ket{0} = \frac{1}{\sqrt{2\pi}} e^{-x^2 / 2} , $$

  and

  $$ \ket{n} = \frac{(a^\dagger)^n}{\sqrt{n!}} \ket{0} , $$

  for $n\in\{1,2,\ldots\}$. These states form an orthonormal set of the Hilbert space
  $L^2 (\RR)$ of square integrable functions. Moreover they are eigenstates of $H$ and $N$
  with $N\ket{n}=n\ket{n}$.
  - Remark :: <<gaussian-integral>> It is well known that the gaussian function which
    defines $\ket{0}$ is already normalized (see [[https://en.wikipedia.org/wiki/Gaussian_integral][gaussian integral]]).
  - Proof :: See [[#exercise-7.4-proof][solution of exercise 7.4]].

** Optical photon quantum computers
The book showed that the beamsplitter $B=e^{-\ii (ab^\dagger-a^\dagger b)}$ acts as
follows on the dual-rail representation

#+name: beamsplitter-dual-rail-basis
#+begin_src sage
  theta = SR.var('theta', domain='real')
  B = matrix([[cos(theta), -sin(theta)], [sin(theta), cos(theta)]])
#+end_src

This essentially follows from these commutation relations:

<<beamsplitter-commutation-relations>>
$$
  BaB^\dagger = a \cos(\theta) + b \sin(\theta)
  \quad \text{and} \quad
  BbB^\dagger = b \cos(\theta) - a \sin(\theta) .
$$

* Exercises
** Exercise 7.1
Using the fact that $x$ and $p$ do not commute, and that in fact $[x,p]=\ii\,\hbar$,
explicitly show that $a^\dagger\,a=H/\hbar\omega-1/2$.

*** Solution
This is just boring algebra which can be done much faster (and more reliably) by /sage/:

#+name: exercise-7.1
#+begin_src sage :results replace :tangle no :cache yes
  assert ad * a == H_qho - 1/2
  "PASSED"
#+end_src

#+RESULTS[38f2058bc713985fbab62335c0887638d917a285]: exercise-7.1
: 'PASSED'

** Exercise 7.2
:PROPERTIES:
:CUSTOM_ID: exercise-7.2
:END:
Given that $[x,p]=\ii\,\hbar$, compute $[a,a^\dagger]$.

*** Solution
The unitless result is $1$:

#+name: exercise-7.2
#+begin_src sage :results replace :tangle no :cache yes
  com(a, ad)
#+end_src

#+RESULTS[78c440463e894f8531e28cce10a7a932478e9b08]: exercise-7.2
: 1

Since the [[unitless-hamiltonian-and-annihilator][creator/annihilator is already unit-less]] the same is true with units.

** Exercise 7.3
Compute $[H,a]$ and use the result to show that if $\ket{\psi}$ is an eigenstate of $H$
with energy $E\geq n\hbar\omega$, then $a^n\ket{\psi}$ is an eigenstate with energy
$E-n\hbar\omega$.

*** Solution
Using $[a^\dagger,a]=-[a,a^\dagger]=-1$ (see [[#exercise-7.2][exercise 7.2]]) we deduce (assuming unit-less quantities)

$$
  [H,a] = [a^\dagger a, a] = (a^\dagger a - a a^\dagger) a = [a^\dagger,a] a = -a .
$$

Using this we get

\begin{align*}
  H a^n \ket{\psi} &= (Ha) a^{n-1} \ket{\psi} \\
  &= ([H,a] + aH)a^{n-1} \ket{\psi} \\
  &= (-a^n + a H a^{n-1}) \ket{\psi} \\
  &= a H a^{n-1} \ket{\psi} - a^n \ket{\psi} .
\end{align*}

Recall that we want to show that $Ha^n\ket{\psi}=(E-n)a^n\ket{\psi}$ for all natural
numbers $n\leq E$. Using the above calculation we can prove this by induction. In fact,
for $n=0$ the assertion is trivial. For $n>0$ we may use the above calculation together
with the assertion for $n-1$:

$$
  H a^n \ket{\psi} = a(E-n+1)a^{n-1}\ket{\psi} - a^n \ket{\psi} = (E-n)a^n\ket{\psi} .
$$

QED.

** Exercise 7.4
Show that $\ket{n}=\frac{(a^\dagger)^n}{\sqrt{n!}}\ket{0}$.

*** Proof
:PROPERTIES:
:CUSTOM_ID: exercise-7.4-proof
:END:

The exercise statement is rather "vague" (I try to be friendly here ðŸ˜‰), so let us prove
some definite statement like the [[spectrum-harmonic-oscillator-1d][theorem about the spectrum of the harmonic oscillator]]
instead.

To find the /ground state/ consider

$$
  \bra{\phi} N \ket{\phi} = \norm{a\phi}^2 \geq 0 .
$$

Equality holds iff

$$
  x \phi(x) + \phi'(x) = \sqrt{2} \cdot (a\phi)(x) = 0 .
$$

This is a linear ordinary differential equation. One solution is given by
$x\mapsto\exp(-x^2/2)$, which can be easily checked by plugging this in. We do not need
this fact (since it follows automatically later on) but the solution is unique up to a
scalar factor, which can be seen by observing that the ODE is equivalent to
$\partial_x\log(\phi(x))=-x$.

The factor $1/\sqrt{2\pi}$ in the definition of $\ket{0}$ [[gaussian-integral][ensures normalization]]. We thus
proved $N\ket{0}=0$. Next let us verify that $\ket{n}$ is an eigenvector. To simplify the
notation let us define $\ket{n'}:=\sqrt{n!}\ket{n}$.

$$
  N\ket{n'} = a^\dagger a (a^\dagger)^n \ket{0} .
$$

By using $[a,a^\dagger]=1$ ([[*Exercise 7.2][exercise 7.2]]) we may move the single $a$ to the right and then
use $a\ket{0}=0$ (this procedure is just simple example of mathematical induction). This
leads to

$$
  N\ket{n'} = n (a^\dagger)^n \ket{0} = n \ket{n'} ,
$$

hence establishing that $\ket{n'}$ (and $\ket{n}$) is an eigenvector for the eigenvalue
$n$. To see that the $1/\sqrt{n!}$ in the definition of $\ket{n}$ is indeed the right
normalization factor use the freshly proved equality $N\ket{n'}=n\ket{n'}$ and consider
(don't forget $[a,a^\dagger]=1$)

$$
  \norm{(n+1)'}^2 = \bra{n'} a a^\dagger \ket{n'}
  = \bra{n'} N + 1 \ket{n'}
  = (n+1) \norm{n'}^2 .
$$

Hence, since $\ket{0}$ is already normalized mathematical induction shows that $\ket{n}$
is normalized too.

It remains to show that the $(\ket{n})$ generate the whole Hilbert space (completeness),
since orthogonality already follows from the fact that they are eigenstates to /different/
eigenvalues of some (unbounded) self-adjoint operator. This essentially boils down to show
that finite linear combinations of the eigenstates are dense in $L^2(\RR)$.

We only sketch the proof since this reaches out to other parts of mathematics. First of
all observe that

$$
  \ket{n}(x) = \frac{1}{\sqrt{2\pi}} \; p_n(x) \; e^{-x^2/2} ,
$$

where the $p_n(x)$ are polynomials which satisfy the recursive relation

$$ p_{n+1}(x)=(2x+\partial_x)p_n(x), \quad p_0(x) = 1 . $$

These are the well-known [[https://en.wikipedia.org/wiki/Hermite_polynomials][hermite polynomials]]. From the recursive relation we directly see
(inductively) the /for our purpose important/ property that $p_n$ has degree $n$ (with
leading factor $2^n$). The density now follows from the following well known results

1. <<ex-7.4-mollification>> The compactly supported continuous functions are dense in
   $L^2(\RR)$. I do not have a good resource on that but one way to see this is by a
   method called /[[https://en.wikipedia.org/wiki/Mollifier][mollification]]/.
2. <<ex-7.4-weierstrass-approx>> For any finite interval $I$ the polynomials on that
   interval are dense in the continuous function on $I$ with respect to the
   $L^\infty$-norm which is stronger than the $L^2$ norm (since the interval is
   finite). This is the [[https://en.wikipedia.org/wiki/Stone%E2%80%93Weierstrass_theorem][Stone-Weierstrass Theorem]].

By [[ex-7.4-weierstrass-approx]] finite linear combinations of eigenstates can approximate any
compactly supported continuous function. Here it is important that any degree is
represented among the eigenstates. It should be obvious that the factor $e^{-x^2/2}$ does
not disturb this argument at all. Now completeness directly follows from
[[ex-7.4-mollification]]. QED.

** Exercise 7.5
Verify that Equations (7.11) and (7.12) are consistent with (7.10) and the normalization
condition $\norm{\ket{n}}^2=1$.

*** Solution
It is not hard to see that (7.11) and (7.12) imply (7.10):

$$
  a^\dagger a \ket{n} = a^\dagger \sqrt{n} \ket{n-1} = n \ket{n} .
$$

The normalization condition is not relevant here. So it is indeed true that it is
consistent with the three equations but for trivial reasons.

** Exercise 7.6 (Eigenstates of photon annihilation)
Prove that a coherent state is an eigenstate of the photon annihilation operator, that is,
show $a\ket{\alpha}=\lambda\ket{\alpha}$ for some constant $\lambda$.

*** Proof
Recall that $a\ket{n}=\sqrt{n}\ket{n-1}$ for $n\geq1$ and $a\ket{0}=0$. Hence

$$
  a\ket{\alpha} = e^{-\abs{\alpha}/2} \sum_n \frac{\alpha^n}{\sqrt{n}} \, a \, \ket{n}
  = e^{-\abs{\alpha}/2} \sum_n \frac{\alpha^{n+1}}{\sqrt{n}} \ket{n}
  = \alpha \ket{\alpha} .
$$

The claim follows with $\lambda=\alpha$. QED.

** Exercise 7.7
Show that the circuit below transforms a dual-rail state by

$$
  \ket{\psi_{\mathrm{out}}} = \begin{bmatrix} e^{\ii\pi} & 0 \\ 0 & 1 \end{bmatrix} \ket{\psi_{\mathrm{in}}} .
$$

if we take the top wire to represent the $\ket{01}$ mode, and $\ket{10}$ the bottom mode,
and the boxed $\pi$ to represent a phase shift by $\pi$.

- Remark :: The book contains a picture showing the circuit.

*** Solution
By definition the circuit acts like this (we use $e^{\ii\pi}=-1$ to simplify notation):

$$
  \ket{0_L} = \ket{01} \mapsto -\ket{0_L}, \quad
  \ket{1_L} = \ket{10} \mapsto \ket{1_L}.
$$

The matrix representing this linear transformation with respect to the basis
$(\ket{0_L},\ket{1_L})$ (the order is important) is

\begin{bmatrix} -1 & 0 \\ 0 & 1 \end{bmatrix}

as desired.

** Exercise 7.8
Show that $P\ket{\alpha}=\ket{\alpha e^{\ii\Delta}}$ where $\ket{\alpha}$ is a coherent
state (note that, in general, $\alpha$ is a complex number!).

*** Proof
The phase shift operator is given by $P\ket{n}=e^{\ii n\Delta}\ket{n}$. Hence, using $\abs{e^{\ii\Delta}}=1$

$$
P\ket{\alpha} = e^{-\abs{\alpha}^2/2} \sum_n \frac{\alpha^n \, e^{\ii n\Delta}}{\sqrt{n!}} \ket{n}
= \ket{\alpha e^{\ii\Delta}} .
$$

QED.

** Exercise 7.9 (Optical Hadamard gate)
Show that the following circuit acts as a Hadamard gate on dual-rail single photon states,
that is, $\ket{01}\mapsto(\ket{01}+\ket{10})/\sqrt{2}$ and
$\ket{10}\mapsto(\ket{01}-\ket{10})/\sqrt{2}$ up to an overall phase.

- Remark :: The book contains a picture showing the circuit.

*** Solution
Assuming evolution from left to right the circuit implements $ZB_{\theta=\pi/4}$ (note
that the phase shift is $Z$ up to a global phase). Below you can see that then the
assertion of the exercise is wrong. We give two alternatives instead.

#+begin_src sage :results replace :tangle no :cache yes
  B0 = B.subs(theta=pi/4)
  B1 = B.subs(theta=-pi/4)

  # This shows that the original circuit does not implement H, not even if we neglect a
  # global phase
  f"sqrt(2)*H != {sqrt(2) * Z * B0}"

  # These alternatives implement the Hadamard gate:
  assert B0 * Z == H
  assert Z * B1 == H
  "PASSED"
#+end_src

#+RESULTS[04d7c5cbd0a5ca296a6d967664b6e4facfdcd1d6]:
: 'sqrt(2)*H != [ 1 -1]\n[-1 -1]'
: 'PASSED'

** Exercise 7.10 (Machâ€“Zehnder interferometer)
Interferometers are optical tools used to measure small phase shifts, which are
constructed from two beamsplitters. Their basic principle of operation can be understood
by this simple exercise.


1. Note that this circuit performs the identity operation:

   $$ B_{\theta=\pi/4}^\dagger \cdot B_{\theta=\pi/4} $$
2. Compute the rotation operation (on dual-rail states) which this circuit performs, as a
   function of the phase shift $\varphi$:

   $$ B_{\theta=\pi/4}^\dagger \cdot R_z(-\varphi) \cdot B_{\theta=\pi/4} $$


- Remark :: The book contains actual circuits drawings instead of algebraic
  expressions. The second expression neglects the global phase (as is common).


*** Solution
Recall that we have $B=B(\theta)=R_y(2\theta)$. Hence $B_{\theta=\pi/4}$ is a rotation
around the y-axis by ninety degrees. This maps the x-axis onto the reversed z-axsis. Hence
the (reversed) z-rotation in the middle effectively acts like a rotation around the x-axis
by an angle $+\varphi$. The net result is $R_x(\varphi)$.

Such reasoning easily leads to subtle errors. Therefore let us verify this using sagemath:

#+begin_src sage :results replace :tangle no :cache yes
  B0 = B.subs(theta=pi/4)
  phi = SR.var('phi', domain='real')

  assert B0.H * Rz.subs(theta=-phi) * B0 == Rx.subs(theta=phi)
  "PASSED"
#+end_src

#+RESULTS[d181afcb2e3cccc86669ae1b88ef476fc645b9a9]:
: 'PASSED'

It worked out ðŸ˜Ž!

** Exercise 7.11
What is $B\ket{2,0}$ for $\theta=\pi/4$?

*** Solution
Following the book we basically identify states with products of creation operators and
then use the [[beamsplitter-commutation-relations][commutation relations]] for the beamsplitter and $B\ket{0,0}=\ket{0,0}$:

$$
  B\ket{2,0} = \frac{1}{\sqrt{2}} B (a^\dagger)^2 \ket{0,0}
  = \frac{1}{\sqrt{2}} \left(a^\dagger \cos(\theta) + b^\dagger \sin(\theta) \right)^2 \ket{0,0} .
$$

Now it helps that $a^\dagger$ and $b^\dagger$ commute, which implies

$$
  \left(a^\dagger \cos(\theta) + b^\dagger \sin(\theta) \right)^2
  = (a^\dagger)^2 \cos(\theta)^2 + (b^\dagger)^2 \sin(\theta)^2 + 2a^\dagger b^\dagger \sin(\theta)\cos(\theta) .
$$

Using $2\sin(x)\cos(x)=\sin(2x)$ we obtain:

$$
  B\ket{2,0} = \cos(\theta)^2 \ket{2,0} + \sin(\theta)^2 \ket{0,2} +
  \frac{\sin(2\theta)}{\sqrt{2}} \ket{1,1} .
$$

Plugging in $\theta=\pi/4$ we obtain

$$
  B_{\theta=\pi/4} \ket{2,0} = \frac{1}{2} \ket{2,0} + \frac{1}{2} \ket{0,2} +
  \frac{1}{\sqrt{2}} \ket{1,1}
$$

** Exercise 7.12 (Quantum beamsplitter with classical inputs)
What is $B\ket{\alpha,\beta}$ where $\ket{\alpha}$ and $\ket{\beta}$ are two coherent
states as in Equation (7.16)? (Hint: recall â€  n that
$\ket{n}=\frac{(a^\dagger)^n}{\sqrt{n!}}\ket{0}$.)

*** Solution
Observe that

$$
  \ket{\alpha} = e^{-\abs{\alpha}^2/2} \sum_n \frac{\alpha^n}{\sqrt{n!}} \ket{n}
  = e^{\alpha a^\dagger - \abs{\alpha}^2/2} \ket{0} .
$$

There is one subtle thing to note here. The operator $(a^\dagger)$ is neither bounded nor
normal. So it is not clear if $e^{\alpha a^\dagger}$ is well defined as an
operator.

Let us give a sketch of how one might make the exponential function rigorous. Let us
define the (large) Hilbert space spanned by the $\ket{n}$ but with scalar product
(implicitly) defined by $\sprod{n}{n}_1=(n!)\inv$. With respect to this Hilbert space
$a^\dagger$ is bounded. Hence we can define $e^{\alpha a^\dagger}$ by the usual
exponential series (we need the space for convergence).

Another way to deal with the problem is to just see it as an abbreviation. In fact, we
only ever apply such operators to $\ket{0,0}$.

In the following let us abreviate $K=e^{-(\abs{\alpha}^2+\abs{\beta}^2)/2}$,
$c=\cos(\theta)$, and $s=\sin(\theta)$. Now let us go on with the calculation:

\begin{align*}
  B \ket{\alpha,\beta}
  &= K B e^{\alpha a^\dagger + \beta b^\dagger} \ket{0,0} \\
  &= K B e^{\alpha a^\dagger + \beta b^\dagger} B^\dagger B \ket{0,0} \\
  &= K \exp(\alpha B a^\dagger B^\dagger + \beta B b^\dagger B^\dagger) \ket{0,0} \\
  &= K \exp(\alpha[ca^\dagger + sb^\dagger] + \beta[cb^\dagger-sa^\dagger]) \ket{0,0} \\
  &= K \exp((\alpha c - \beta s)a^\dagger + (\alpha s + \beta c)b^\dagger) \ket{0,0} \\
  & = \ket{\alpha c - \beta s, \alpha s + \beta c} .
\end{align*}

Hence the operation of $B$ on coherent states is again given by a rotation matrix:

$$
  B: \begin{pmatrix} \alpha \\ \beta \end{pmatrix} \mapsto
  \begin{bmatrix} c & -s \\ s & c \end{bmatrix} \begin{pmatrix} \alpha \\ \beta \end{pmatrix} .
$$
